eIris/proofmode/telescopes.v
@@ -13,10 +13,10 @@ Local Set Polymorphic Inductive Cumulativity.
 Local Unset Universe Minimization ToSet.
 
 (** Telescopes *)
-Inductive teleC@{u} : Type@{max(Set, u+1)} :=
+Inductive teleC : Type :=
   | TeleCO : teleC
-  | TeleCC (X : Type@{u}) (t : teleC) : teleC
-  | TeleCS {X : Type@{u}} (binder : X → teleC) : teleC.
+  | TeleCC (X : ofe) (t : teleC) : teleC
+  | TeleCS {X : Type} (binder : X → teleC) : teleC.
 
 Check TeleCC.
 
@@ -32,8 +32,6 @@ Fixpoint teleC_fun (TT : teleC) (T : Type) : Type :=
 
 Notation "TT -tc> A" :=
   (teleC_fun TT A) (at level 99, A at level 200, right associativity).
-
-Compute ((TeleCC ofe (TeleCS (fun (x : nat) => TeleCS (fun _ : vec bool x => TeleCO)))) -tc> Prop).
 
 (** An eliminator for elements of [tele_fun].
     We use a [fix] because, for some reason, that makes stuff print nicer
@@ -55,6 +53,107 @@ Record teleC_arg_cons {X : Type} (f : X → Type) : Type := TeleCArgCons
     teleC_arg_tail : f teleC_arg_head }.
 Global Arguments TeleCArgCons {_ _} _ _.
 
+Section Args_Cons_OFE.
+  (** * SigmaT type *)
+  (** Ofe for [teleC_arg_cons]. The first component must be discrete and use Leibniz
+  equality, while the second component might be any OFE. *)
+  Import EqNotations.
+
+  Context {A : Type} {P : A → ofe}.
+  Implicit Types x : teleC_arg_cons P.
+
+  (**
+    The distance for [{ a : A & P }] uses Leibniz equality on [A] to
+    transport the second components to the same type,
+    and then step-indexed distance on the second component.
+    Unlike in the topos of trees, with (C)OFEs we cannot use step-indexed equality
+    on the first component.
+  *)
+  Local Instance teleC_arg_cons_dist : Dist (teleC_arg_cons P) := λ n x1 x2,
+    ∃ Heq : teleC_arg_head P x1 = teleC_arg_head P x2, rew Heq in teleC_arg_tail P x1 ≡{n}≡ teleC_arg_tail P x2.
+
+  (**
+    Usually we'd give a direct definition, and show it equivalent to
+    [∀ n, x1 ≡{n}≡ x2] when proving the [equiv_dist] OFE axiom.
+    But here the equivalence requires UIP — see [sigT_equiv_eq_alt].
+    By defining [equiv] in terms of [dist], we can define an OFE
+    without assuming UIP, at the cost of complex reasoning on [equiv].
+  *)
+  Local Instance teleC_arg_cons_equiv : Equiv (teleC_arg_cons P) := λ x1 x2,
+    ∀ n, x1 ≡{n}≡ x2.
+
+  (** Unfolding lemmas.
+      Written with [↔] not [=] to avoid https://github.com/coq/coq/issues/3814. *)
+  Definition teleC_arg_cons_equiv_eq x1 x2 : (x1 ≡ x2) ↔ ∀ n, x1 ≡{n}≡ x2 :=
+      reflexivity _.
+
+  Definition teleC_arg_cons_dist_eq x1 x2 n : (x1 ≡{n}≡ x2) ↔
+    ∃ Heq : teleC_arg_head P x1 = teleC_arg_head P x2, (rew Heq in teleC_arg_tail P x1) ≡{n}≡ teleC_arg_tail P x2 :=
+      reflexivity _.
+
+  Definition teleC_arg_cons_dist_proj1 n {x y} : x ≡{n}≡ y → teleC_arg_head P x = teleC_arg_head P y := proj1_ex.
+  Definition teleC_arg_cons_equiv_proj1 {x y} : x ≡ y → teleC_arg_head P x = teleC_arg_head P y := λ H, proj1_ex (H 0).
+
+  Definition teleC_arg_cons_ofe_mixin : OfeMixin (teleC_arg_cons P).
+  Proof.
+    split => // n.
+    - split; hnf; setoid_rewrite teleC_arg_cons_dist_eq.
+      + intros. by exists eq_refl.
+      + move => [xa x] [ya y] /=. destruct 1 as [-> Heq].
+        by exists eq_refl.
+      + move => [xa x] [ya y] [za z] /=.
+        destruct 1 as [-> Heq1].
+        destruct 1 as [-> Heq2]. exists eq_refl => /=. by trans y.
+    - setoid_rewrite teleC_arg_cons_dist_eq.
+      move => m [xa x] [ya y] /=. destruct 1 as [-> Heq].
+      exists eq_refl. by eapply dist_dist_later.
+  Qed.
+
+  Canonical Structure teleC_arg_consO : ofe := Ofe (teleC_arg_cons P) teleC_arg_cons_ofe_mixin.
+
+  Lemma teleC_arg_cons_equiv_eq_alt `{!∀ a b : A, ProofIrrel (a = b)} x1 x2 :
+    x1 ≡ x2 ↔
+    ∃ Heq : teleC_arg_head P x1 = teleC_arg_head P x2, rew Heq in teleC_arg_tail P x1 ≡ teleC_arg_tail P x2.
+  Proof.
+    setoid_rewrite equiv_dist; setoid_rewrite teleC_arg_cons_dist_eq; split => Heq.
+    - move: (Heq 0) => [H0eq1 _].
+      exists H0eq1 => n. move: (Heq n) => [] Hneq1.
+      by rewrite (proof_irrel H0eq1 Hneq1).
+    - move: Heq => [Heq1 Heqn2] n. by exists Heq1.
+  Qed.
+
+  (** [teleC_arg_head] is non-expansive and proper. *)
+  Global Instance teleC_arg_head_ne : NonExpansive (teleC_arg_head P : teleC_arg_consO → leibnizO A).
+  Proof. solve_proper. Qed.
+
+  Global Instance teleC_arg_head_proper : Proper ((≡) ==> (≡)) (teleC_arg_head P : teleC_arg_consO → leibnizO A).
+  Proof. apply ne_proper, teleC_arg_head_ne. Qed.
+
+  (** [teleC_arg_tail] is "non-expansive"; the properness lemma [teleC_arg_tail_ne] requires UIP. *)
+  Lemma teleC_arg_tail_ne n (x1 x2 : teleC_arg_consO) (Heq : x1 ≡{n}≡ x2) :
+    rew (teleC_arg_cons_dist_proj1 n Heq) in teleC_arg_tail P x1 ≡{n}≡ teleC_arg_tail P x2.
+  Proof. by destruct Heq. Qed.
+
+  Lemma teleC_arg_tail_proper `{!∀ a b : A, ProofIrrel (a = b)} (x1 x2 : teleC_arg_consO) (Heqs : x1 ≡ x2):
+    rew (teleC_arg_cons_equiv_proj1 Heqs) in teleC_arg_tail P x1 ≡ teleC_arg_tail P x2.
+  Proof.
+    move: x1 x2 Heqs => [a1 x1] [a2 x2] Heqs.
+    case: (proj1 (teleC_arg_cons_equiv_eq_alt _ _) Heqs) => /=. intros ->.
+    rewrite (proof_irrel (teleC_arg_cons_equiv_proj1 Heqs) eq_refl) /=. done.
+  Qed.
+
+  Implicit Types (c : chain teleC_arg_consO).
+
+  Global Instance teleC_arg_cons_discrete x : Discrete (teleC_arg_tail P x) → Discrete x.
+  Proof.
+    move: x => [xa x] ? [ya y] [] /=; intros -> => /= Hxy n.
+    exists eq_refl => /=. apply equiv_dist, (discrete _), Hxy.
+  Qed.
+
+  Global Instance teleC_arg_cons_ofe_discrete : (∀ a, OfeDiscrete (P a)) → OfeDiscrete teleC_arg_consO.
+  Proof. intros ??. apply _. Qed.
+End Args_Cons_OFE.
+
 (** A sigma-like type for an "element" of a telescope, i.e. the data it
   takes to get a [T] from a [TT -t> T]. *)
 Fixpoint teleC_arg@{u} (t : teleC@{u}) : Type@{u} :=
@@ -64,6 +163,14 @@ Fixpoint teleC_arg@{u} (t : teleC@{u}) : Type@{u} :=
   | TeleCS f => teleC_arg_cons (λ x, teleC_arg (f x))
   end.
 Global Arguments teleC_arg _ : simpl never.
+
+Fixpoint teleC_argO (t : teleC) : ofe :=
+  match t with
+  | TeleCO => unit
+  | TeleCC C t => prodO C (teleC_argO t)
+  | TeleCS f => teleC_arg_cons (λ x, teleC_argO (f x))
+  end.
+Global Arguments teleC_argO _ : simpl never.
 
 Compute teleC_arg (TeleCC ofe (TeleCS (fun (x : nat) => TeleCS (fun _ : vec bool x => TeleCO)))).
 
